\documentclass{ximera}
\input{../lessonplanheader.tex}

\title{Multiplicative inverses using Wilson's Theorem}
\begin{document}
\begin{abstract}
\end{abstract}
\maketitle

%%%%%%%%%%%%%%%%%%%%%%%%%%

\begin{obj}
\item Use Wilson's Theorem to find the least nonnegative residue modulo a prime
\end{obj}




First, some important algebra  for multiplicative inverses
\begin{example}
  \begin{enumerate}
    \item  Let $n$ be an odd positive integer. Then \[2\left(\frac{n+1}{2}\right)=n+1\equiv 1\pmod{n}.\] So $\frac{n+1}{2}$ is the multiplicative inverse of $2$ modulo $n$. 
    \begin{tps}
      Why is $\left(\frac{n+1}{2},n\right)=1$?
    \end{tps}

    We also have that $n-\frac{n+1}{2}= \frac{n-1}{2}$ and $n-2\equiv -2\pmod{n},$ so $\frac{n-1}{2}$ is the multiplicative inverse of $n-2$ modulo $n.$ Another way to see this is 
    \[-2\left(\frac{n-1}{2}\right)=-n+1\equiv 1\pmod{n}.\] 

    \item Let $m$ and $n$ be positive integers such that $n\equiv 1\pmod m.$ Then there exists $k\in\Z$ such that $n=mk+1$ by the \nameref{defn:mod-equiv-all}. Then 
    \[-m\left(\frac{n-1}{m}\right)=-n+1\equiv 1\pmod{n}.\]

    \item Let $m$ and $n$ be positive integers such that $n\equiv -1\pmod m.$ Then there exists $k\in\Z$ such that $n=mk-1$ by definition. Then 
    \[m\left(\frac{n+1}{m}\right)=n+1\equiv 1\pmod{n}.\]
  \end{enumerate}

\end{example}


\begin{example}
  \begin{enumerate}
    \item  Practice with Wilson's Theorem: 
    Find  $\frac{31!}{23!} \pmod{11}.$
    \begin{align*}
    x\equiv \frac{31!}{23!}	 & \equiv  24(25)(26)(27)(28)(29)(30)(31) \pmod{11}\\
          & \equiv  2(3)(4)(5)(6)(7)(8)(9) \pmod{11}.
    \end{align*}
    Then $-x\equiv 10! \equiv -1\pmod{11}.$ Therefore, $x\equiv 1\pmod{11}.$

    \item Let $p$ be an odd prime $p,$ then $2(p-3)!\equiv -1 \pmod{p}$.
    
    \begin{proof}
    Let $p$ be an odd prime, then $(p-1)!\equiv -1\pmod{p}$ by Wilson's Theorem. Multiplying both sides of the congruence by $-1$ gives $(p-2)!\equiv 1\pmod{p}.$ Since $(p-2)!=(p-3)!(p-2)$ by the definition of factorial, $p-2\equiv -2\pmod{p}$ is the multiplicative inverse of $(p-3)!$ modulo $p.$ Thus, 
    \begin{align*}
    -2(p-3)!	&\equiv 1\pmod{p}\\
    2(p-3)!	 & \equiv  -1\pmod{p}.\qedhere
    \end{align*}
    \end{proof}
  \end{enumerate}

\end{example}

\end{document}
