\documentclass{ximera}
\input{../lessonplanheader.tex}

<<<<<<< Updated upstream
\title{Introduction to modular arithmetic}
=======
\title{Equivalent of equivalence modulo $m$}
>>>>>>> Stashed changes
\begin{document}
\begin{abstract}
\end{abstract}
\maketitle

%%%%%%%%%%%%%%%%%%%%%%%%%%
\begin{obj}
\item Prove that congruence modulo $m$ is an equivalence relation on $\Z$.
\item Define a complete residue system.
\item Practice using modular arithmetic.
\end{obj}
<<<<<<< Updated upstream


\begin{instructorNotes}
=======
>>>>>>> Stashed changes
    
\begin{pre}
    \item[Read] Strayer, Section 2.1 through Example 1.
    \item[Turn in] The book concludes the section with a caution about division. It states that $6a\equiv 6b \pmod 3$ for all integers $a$ and $b$. Explain why this is true.
    
    
    \begin{solution}
        Since $3\mid 6a-6b=3(2a-2b),$ $6a\equiv 6b \pmod 3$ for all integers $a$ and $b$.
    \end{solution}
    \end{pre}

<<<<<<< Updated upstream
\end{instructorNotes}



=======
>>>>>>> Stashed changes
\begin{defn}[divisibility definition of $a\equiv b \pmod{m}$]\label{defn:mod-divides} Let $a,b,m\in\Z$ with $m>0.$
We say that $a$ is \emph{congruent to $b$ modulo $m$} and write $a \equiv b \pmod{m}$ if $m\mid b-a$, and $m$ is said to be the \emph{modulus of the congruence}. The notation $a\not\equiv b\pmod m$ means $a$ is not congruent to $b$ modulo $m,$ or $a$ is \emph{incongruent to $b$ modulo $m$.} 
\end{defn}

\begin{defn}[remainder definition of $a\equiv b \pmod{m}$]\label{defn:mod-remainder} Let $a,b,m\in\Z$ with $m>0.$ We say that $a$ is congruent to $b$ modulo $m$ if $a$ and $b$ have the same remainder when divided by $m$. 
\end{defn}
Be careful with this idea and negative values. Make sure you understand why $-2\equiv 1\pmod{3}$ or $-10\equiv 4\pmod{7}$.

\begin{proposition}[Definitions of congruence modulo $m$ are equivalent]\label{prop:mod-defn:equiv}
These two definitions are equivalent. That is, for $a,b,m\in\Z$ with $m>0,$ $m\mid b-a$ if and only if $a$ and $b$ have the same remainder when divided by $m$.
\end{proposition}

\begin{proof}
Let $a,b,m\in\Z$ with $m> 0.$ By the \nameref{div-alg}, there exists $q_1,q_2,r_1,r_2\in\Z$ such that \begin{align*}
                    a & q_1 m +r_1, 0\leq r_1< m, \textnormal{ and }\\
                    b & q_2 m +r_2, 0\leq r_2< m.
                \end{align*}
            
            
                If $m\mid b-a,$ then by definition, there exists $k\in\Z$ such that $mk=b-a.$ Thus, $mk=q_2 m+r_2-q_1 m-r_1.$ Rearranging, we get 
                $m(k-q_2+q_1)=r_2-r_1$ and $m\mid r_2-r_1.$ Since 
                $0\leq r_1< m, 0\leq r_2< m,$ we have 
                $-m< r_2-r_1< m.$ Thus, $r_2-r_1=0,$ so $a$ and $b$ have the same remainder when divided by $m$.
            

            
                In the other direction, if $r_1=r_2,$ then $a-b=q_1 m-q_2 m=m(q_1-q_2).$ Thus, $m\mid a-b.$
\end{proof}

\begin{example}
 We will eventually find a function that generates all integers solutions to the equation $a^2+b^2=c^2$ (this can be done with only divisibility, so feel free to try for yourself after class).
 
 Modular arithmetic allows us to say a few things about solutions. 
 \begin{description}
 \item[First, let's look at $\!\pmod 2$.] Note that $0^2\equiv 0 \pmod 2$ and $1^2\equiv 1 \pmod 2$.

\begin{description}
 \item[Case 1: $c^2\equiv 0 \pmod 2$] In this case, $c\equiv 0\pmod 2$ and either $1^2+1^2\equiv 0\pmod 2$ or $0^2+0^2\equiv 0\pmod 2$. So, we know $a\equiv b\pmod 2.$ \emph{(Note: $\!\pmod 4$ will eliminate the $a\equiv b\equiv 1 \pmod 2$ case)}
  \item[Case 2: $c^2\equiv 1 \pmod 2$] In this case, $c\equiv 1\pmod 2$ and either $0^2+1^2\equiv 1\pmod 2$. So, we know $a\not\equiv b\pmod 2.$
\end{description}

\item[Let's start with $\!\pmod 3$.] Note that $0^2\equiv 0 \pmod 3$, $1^2\equiv 1 \pmod 3$, and $2^2\equiv 1 \pmod 3$.
\end{description} 

\begin{description}
 \item[Case 1: $c^2\equiv 0 \pmod 3$.] In this case, $c\equiv 0\pmod 3$ and $0^2+0^2\equiv 0\pmod 3$. So, we know $a\equiv b\equiv c\equiv 0\pmod 3.$ 
  \item[Case 2: $c^2\equiv 1 \pmod 3$.] In this case, $c$ could be $1$ or $2$ modulo $3$. We also know $0^2+1^2\equiv 1\pmod 3$, so  $a\not\equiv b\pmod 3.$
  \item[Case 3: $c^2\equiv 2 \pmod 3$] has no solutions.
\end{description}

So at least one of $a,b,c$ is even, and at least one is divisible by $3$.
\end{example}

We can use the idea of congruences to simplify divisibility arguments, as well as nonlinear Diophantine equations.






\end{document}
