\documentclass{ximera}
\input{../lessonplanheader.tex}

\title{Legendre symbol}
\begin{document}
\begin{abstract}
\end{abstract}
\maketitle

%%%%%%%%%%%%%%%%%%%%%%%%%%

\begin{obj}
    \item Define the Legendre symbol
    \item Prove basic facts about the Legendre symbol
    \item Use the definition and basic facts to find the Legendre symbol for specific examples
\end{obj}


\begin{pre}
<<<<<<< Updated upstream
    \item[Reading:] Strayer Section 4.2 through Example 4
=======
    \item[Read:] Strayer Section 4.2 through Example 4
>>>>>>> Stashed changes
    \item[Turn in:] Exercise 12
     Use Euler's Criterion to evaluate the following Legendre symbols 
	\begin{enumerate}
 		\item $\left(\frac{11}{23}\right)$
		
		\begin{solution}
 			$\left(\frac{11}{23}\right)\equiv 11^{(23-1)/2}\equiv 11^{11}\pmod{23}$ By Euler's Criterion. Then
			\[11^{11}\equiv (11^{2})^{5}(11)\equiv 6^5(11)\equiv (6^2)(6^3)(11)\equiv (13)(9)(11)\equiv(-90)(11)\equiv -1\pmod{23}\]
		\end{solution}
		
		\item $\left(\frac{-6}{11}\right)$
		
		\begin{solution}
 			$\left(\frac{-6}{11}\right)\equiv (-6)^{(11-1)/2}\equiv (-6)^{5}\pmod{11}$ By Euler's Criterion. Then
			\[(-6)^{5}\equiv ((6)^{2})^{2}(-6)\equiv 3^2(-6)\equiv -54 \equiv 1\pmod{11}\]
		\end{solution}
	\end{enumerate}
 

<<<<<<< Updated upstream
    \end{pre}


%%%%%%%%%%%%%%%%%%%%%%%%%%
\subsection{Quiz (15 minutes)}
%%%%%%%%%%%%%%%%%%%%%%%%%%
Technical difficults with printer and projector.

%%%%%%%%%%%%%%%%%%%%%%%%%%
\subsection{Legendre symbol (35 minutes)}
%%%%%%%%%%%%%%%%%%%%%%%%%%
=======
\end{pre}


>>>>>>> Stashed changes

\begin{definition}[Legendre symbol]\label{defn:legendre}
    Let $p$ be an odd prime number and let $a\in\Z$ with $p\nmid a$. The \emph{Legendre symbol}, denoted $\legendre{a}{p}$, is
        \[
            \legendre{a}{p}=
            \begin{cases}
                1, & \text{ if $a$ is a quadratic residue modulo $p$} \\
                -1, & \text{ if $a$ is a quadratic nonresidue modulo $p$} 
            \end{cases}
        \]
\end{definition}

\begin{theorem}[Euler's Criterion]\label{thm:euler-quads}
    Let $p$ be an odd prime and $a\in\Z$ with $p\nmid a.$ Then \[\legendre{a}{p}\equiv a^{(p-1)/2}\pmod{p}\]
\end{theorem}

We will not prove this today, but we will use it to go over the solution to the reading assignment and to prove the following proposition.

<<<<<<< Updated upstream
\begin{proposition}[Proposition 4.5]\label{prop:legendre-facts}
	Let $p$ be an odd prime number and $a,b\in\Z$ with $p\nmid a$ and $p\nmid b.$ Then 
	\begin{enumerate}[label=(\alph*)]
=======
\begin{proposition}\label{prop:legendre-facts}
	Let $p$ be an odd prime number and $a,b\in\Z$ with $p\nmid a$ and $p\nmid b.$ Then 
	\begin{enumerate}
>>>>>>> Stashed changes
		\item $\legendre{a^2}{p}=1$ \label{squares-are-square}
		\item If $a\equiv b\pmod{p}$ then $\legendre{a}{p}=\legendre{b}{p}$ \label{legendre-respects-mod}
		\item $\legendre{ab}{p}=\legendre{a}{p}\legendre{b}{p}$ \label{legendre-mult}
	\end{enumerate}
\end{proposition}


\begin{proof}
    Let $p$ be an odd prime number and $a,b\in\Z$ with $p\nmid a$ and $p\nmid b.$ Then $a^2$ is a quadratic residue modulo $p,$ by definition, so $\legendre{a^2}{p}=1$ by the definition of the Legendre symbol.

    If $a\equiv b\pmod{p},$ then either both $a$ and $b$ are quadratic residues modulo $p$ or both $a$ and $b$ are quadratic nonresidues modulo $p.$ Thus $\legendre{a}{p}=\legendre{b}{p}.$

    For the last part, \nameref{thm:euler-quads} gives \[\legendre{ab}{p}\equiv (ab)^{(p-1)/2}\equiv (a^{(p-1)/2})(b^{(p-1)/2})\equiv \legendre{a}{p}\legendre{b}{p}\pmod{p}\]
\end{proof}

<<<<<<< Updated upstream
=======
\begin{remark}
	Some sources define $\legendre{a}{p}=0$ when $p\mid a.$ In this case,  Let $p$ be an odd prime and $a\in\Z$.
	If $p\mid a,$ then $a^{(p-1)/2}\equiv 0^{(p-1)/2}\equiv 0\equiv\legendre{a}{p}\pmod{p}.$
\end{remark}


\begin{theorem}\label{thm:residue-neg1}
	Let $p$ be an odd prime number. Then 
	\[
		\legendre{-1}{p}=
			\begin{cases}
 				1, & p\equiv 1\pmod{4}\\
				-1, & p\equiv 3\pmod{4}
			\end{cases}.
	\]
	\begin{proof}
		Let $p$ be an odd prime number. Then from \nameref{thm:euler-quads}, $\legendre{-1}{p}\equiv (-1)^{(p-1)/2}\pmod{p}.$ Since both values are $\pm1,$ we can say $\legendre{-1}{p}=(-1)^{(p-1)/2}.$
	
		If $p\equiv 1\pmod{4},$ then there exists $k\in\Z$ such that $p=4k+1.$ Thus, $\frac{p-1}{2}=2k$ and 
			\[
				\legendre{-1}{p}=(-1)^{(p-1)/2}=(-1)^{2k}=1.
			\]
		
		If $p\equiv 3\pmod{4},$ then there exists $k\in\Z$ such that $p=4k+3.$ Thus, $\frac{p-1}{2}=2k+1$ and 
			\[
				\legendre{-1}{p}=(-1)^{(p-1)/2}=(-1)^{2k+1}=-1.
			\]
	\end{proof}
\end{theorem}


%%%%%%%%%%%%%%%%%%%%%%%%%%
>>>>>>> Stashed changes


\end{document}
