\documentclass{ximera}
\input{../lessonplanheader.tex}

<<<<<<< Updated upstream
\title{More modular arithmetics}
=======
\title{Modular arithmetic facts}
>>>>>>> Stashed changes
\begin{document}
\begin{abstract}
\end{abstract}
\maketitle

%%%%%%%%%%%%%%%%%%%%%%%%%%

\begin{obj}
\item Prove basic facts about modular arithmetic.
%  \item Understand gaps in argument and writing of proof of Exercise 83. Give classmates useful feedback on their proofs.
\end{obj}

\begin{defn}[$a\equiv b\pmod{m}$]\label{defn:mod-equiv-all}
Let $a,b,m\in\Z$ with $m>0.$ From Friday, we have the following equivalent definitions of congruence modulo $m:$
\begin{enumerate}
 \item $a\equiv b \pmod m$ if and only if\footnote{all definitions are if and only if} $m\mid b-a$ (standard definition, generalizing even/odd based on divisibility)
 \item $a\equiv b \pmod m$ if and only if $a$ and $b$ have the same remainder with divided by $m.$ That is, That is, there exists unique $q_1,q_2,r\in\Z$ such that  $a=mq_1+r,\   b=mq_2+r,\  0\leq r<m.$ (definition generalizing even/odd based on remainder)
\item $a\equiv b\pmod m$ if and only if $a$ and $b$ differ by a multiple of $m.$ That is, $b=a+mk$ for some $k\in\Z.$ (arithmetic progression definition)
\end{enumerate}
\end{defn}

Different statements of the definition will be useful in different situations

\begin{proposition}\label{prop:equiv-arith}%[Restatement of Propositions 2.1, 2.4, and 2.5]
 Let $a,b,c,d,m\in\Z$ with $m>0,$ then:
\begin{enumerate}
\item $a\equiv b \pmod{m}$ and $b\equiv c \pmod{m}$ implies $a\equiv c \pmod{m}$
\item\label{equiv-add} $a\equiv b \pmod{m}$ and $c\equiv d \pmod{m}$ implies $a+c \equiv b+d \pmod{m}$ 
\item\label{equiv-multiply} $a\equiv b\pmod{m}$ and $c\equiv d \pmod{m}$ implies $ac\equiv bd \pmod{m}$.
\item $a\equiv b \pmod{m}$ and $d\mid m$, $d>0$ implies $a\equiv b \pmod{d}$
\item\label{equiv-upmod} $a\equiv b \pmod{m}$ implies $ac\equiv bc \pmod{mc}$ for $c>0$.
\end{enumerate}
\end{proposition}
\begin{proof}
  Let $a,b,c,d,m\in\Z$ with $m>0.$
  
\begin{enumerate}
  \item Assume $a\equiv b \pmod{m}$ and $b\equiv c \pmod{m}.$ Then using the second definition of equivalence, there exists $q_1,q_2,q_3,r\in\Z$ such that 
  \begin{align*}
    a&=mq_1+r, \qquad 0\leq r<m,\\
    b&=mq_2+r, \qquad 0\leq r<m,\\
    c&=mq_3+r, \qquad 0\leq r<m. 
  \end{align*}
  Thus, $a$ and $c$ have the same remainder when divided by $m,$ so $a\equiv c\pmod m.$

  \item[\ref{equiv-add}/\ref{equiv-multiply}] \addtocounter{enumi}{2}
  Assume $a\equiv b \pmod{m}$ and $c\equiv d \pmod{m}.$ Then by the third definition of equivalence, there exists $j,k\in\Z$ such that $b=a+mj$ and $d=c+mk.$ Thus, 
  \begin{align*}
    b+d&=a+c+m(j+k), \qquad\qquad\textnormal{and}\\
    bd &= ac+m(ak+cj+mjk).
  \end{align*}
  Thus, $a+c\equiv b+d\pmod m$ and $ac=bd\pmod m.$

  \item Assume $a\equiv b \pmod{m},$ and $d>0$ with $d\mid m.$ From the first definition of equivalence modulo $m,$ $m\mid b-a$. Since division is transitive, $d\mid b-a,$ so $a\equiv b\pmod d.$

  \item Assume $a\equiv b \pmod{m},$ and $c>0.$ From the third definition of equivalence modulo $m,$ there exists $k\in\Z$ such that $b=a+mk.$ Thus, $bc=ac+mck,$ so $ac\equiv bc \pmod{mc}.$ \qedhere
\end{enumerate}
\end{proof}

\begin{example}
Note that $2\equiv 5 \pmod 3$. Then $4\equiv 10 \pmod 3$ by \hyperref[equiv-multiply]{Proposition \ref{prop:equiv-arith}\ref{equiv-multiply}}, since $2\equiv 2\pmod 3.$ From part \ref{equiv-upmod}, $4\equiv 10 \pmod 6,$ but $2\not\equiv 5\pmod 6.$ 
\end{example}

\end{document}
