\documentclass{../ximera}
\input{../lessonplanheader.tex}

\title{Quadratic residue of $-1$}
\begin{document}
\begin{abstract}
\end{abstract}
\maketitle

%%%%%%%%%%%%%%%%%%%%%%%%%%

\begin{obj}
    \item Prove \nameref{thm:euler-quads}
	\item Classify when $-1$ is a quadratic residue modulo an odd prime
\end{obj}


\begin{pre}
    \item[Reading] None
\end{pre}

%%%%%%%%%%%%%%%%%%%%%%%%%%
\subsection{Proof of Euler's Criterion}
%%%%%%%%%%%%%%%%%%%%%%%%%%

We will prove \nameref{thm:euler-quads}. 

\begin{thm*}[Euler's Criterion]
    Let $p$ be an odd prime and $a\in\Z$ with $p\nmid a.$ Then \[\legendre{a}{p}\equiv a^{(p-1)/2}\pmod{p}\]
\end{thm*}

\begin{proof}
	Let $p$ be an odd prime and $a\in\Z$ with $p\nmid a.$ If there exists $b\in\Z$ such that $b^2\equiv a\pmod{p},$ then $\legendre{a}{p}=1$ by \hyperref[defn:legendre]{definition}.
	Note that \[a^{(p-1)/2}\equiv (b^2){(p-1)/2}\equiv b^{p-1}\equiv 1\pmod{p}\]
	by \nameref{FlT}. Thus $\legendre{a}{p}\equiv a^{(p-1)/2}\pmod{p}.$
	
	If $a$ is a quadratic nonresidue modulo $p,$ consider the \hyperref[defn:reduced-res-sys]{reduced residue system} $\{1,2,\dots,p-1\}.$ For each element $c$ of the list, there exists a unique element $d$, also on the list, such that $cd\equiv a\pmod{p}$ by \hyperref[thm:lin-cong-solutions]{Theorem 2.6} since $(a,p)=1$. Since $a$ is a quadratic nonresidue by assumption, $c\not\equiv d\pmod{p}.$ Thus, there are $\frac{p-1}{2}$ pairs $c,d$ where $cd\equiv a\pmod{p}.$ Thus, 
		\[
			-1\equiv (p-1)! \equiv a^{(p-1)/2}\pmod{p}
		\]
	by \nameref{Wilson}. Since $a$ is a quadratic nonresidue modulo $p,$ $\legendre{a}{p}=-1\equiv a^{(p-1)/2}\pmod{p}.$
\end{proof}

\begin{remark}
	Some sources define $\legendre{a}{p}=0$ when $p\mid a.$ In this case,  Let $p$ be an odd prime and $a\in\Z$.
	If $p\mid a,$ then $a^{(p-1)/2}\equiv 0^{(p-1)/2}\equiv 0\equiv\legendre{a}{p}\pmod{p}.$
\end{remark}

%%%%%%%%%%%%%%%%%%%%%%%%%%
\subsection{When is $-1$ a quadratic residue?}
%%%%%%%%%%%%%%%%%%%%%%%%%%

\begin{thm*}[Theorem 4.6]\label{thm:residue-neg1}
	Let $p$ be an odd prime number. Then 
	\[
		\legendre{-1}{p}=
			\begin{cases}
 				1, & p\equiv 1\pmod{4}\\
				-1, & p\equiv 3\pmod{4}
			\end{cases}.
	\]
\end{thm*}

\begin{proof}
	Let $p$ be an odd prime number. Then from \nameref{thm:euler-quads}, $\legendre{-1}{p}\equiv (-1)^{(p-1)/2}\pmod{p}.$ Since both values are $\pm1,$ we can say $\legendre{-1}{p}=(-1)^{(p-1)/2}.$

	If $p\equiv 1\pmod{4},$ then there exists $k\in\Z$ such that $p=4k+1.$ Thus, $\frac{p-1}{2}=2k$ and 
		\[
			\legendre{-1}{p}=(-1)^{(p-1)/2}=(-1)^{2k}=1.
		\]
	
	If $p\equiv 3\pmod{4},$ then there exists $k\in\Z$ such that $p=4k+3.$ Thus, $\frac{p-1}{2}=2k+1$ and 
		\[
			\legendre{-1}{p}=(-1)^{(p-1)/2}=(-1)^{2k+1}=-1.
		\]
\end{proof}
%%%%%%%%%%%%%%%%%%%%%%%%%%


\end{document}
