\documentclass{ximera}
\input{../lessonplanheader.tex}

\title{Sum of Two Squares}
\begin{document}
\begin{abstract}
\end{abstract}
\maketitle

%%%%%%%%%%%%%%%%%%%%%%%%%%

\begin{pre}
    \item[Reading] None
\end{pre}


\begin{theorem}\label{thm:express-sum-sqrs}
	Let $n\in\mathbb{Z}$ with $n>0$. Then $n$ is expressible as the sum of two squares if and only if every prime factor congruent to $3$ modulo  $4$ occurs to an even power in the prime factorization of $n$.

\begin{proof}
	($\Leftarrow$) Assume that every prime factor of $n$ congruent to $3$ modulo $4$ occurs to an even power in the prime factorization of $n$. Then $n$ can be written as $n=m^2p_1p_2\dots  p_r$ where $m\in\mathbb{Z}$ and $p_1,p_2,\dots,p_r$ are distinct prime numbers equal to $2$ or equivalent to $1$ modulo $4$. Now, $m^2=m^2+0^2$, so is expressible as the sum of two squares, and each $p_1$ is also expressible as the sum of two squares by the theorem labeled Primes as Sums of Squares. Thus, by the first theorem of the day, $n$ is expressible as the sum of two squares.
	
	($\Rightarrow$) Assume that $p$ is an odd prime number and that $p^{2i+1},i\in\mathbb{Z}$ occurs in the prime factorization of $n$. We will show that $p\equiv 1 \pmod 4$. Since $n$ is expressible as the sum of two squares of integers, there exist $x,y\in\mathbb{Z}$ such that $n=x^2+y^2.$ Let $(x,y)=d, a=\frac{x}{d},b=\frac{y}{d}$ and  $m=\frac{n}{d^2}$. Then $(a,b)=1$ and $a^2+b^2=m$. Let $p^j,j\in\mathbb{Z}$ be the largest power of $p$ dividing $d$. Then $p^{(2i-1)-2j}\mid m$; since $(2i+1)-2j)\geq 1$, we have $p\mid m$. Now, $p\nmid a$ since $(a,b)=1$. Thus, there exists $z\in\mathbb{Z}$ such that $az\equiv b \pmod p$. Then $m=a^2+b^2\equiv a^2+(az)^2\equiv a^2(1+z^2)\pmod p$.
	 
	Since $p\mid m$, we have \[a^2(1+z^2)\equiv 0\pmod p\] or $p\mid a^2(1+z^2)$ or $z\equiv -1 \pmod p$. Thus, $-1$ is a quadratic residue modulo $p$, so $p\equiv 1 \pmod 4$. By contrapositive, any prime factor congruent to $3$ modulo $4$ occurs to an even power in the prime factorization of $n$ as desired.
	 
	
   \end{proof}
\end{theorem}




\end{document}
